update ArrayN

SciLean/Data/ArrayN.lean
@@ -1,11 +1,67 @@
+import Aesop
+import SciLean.Util.SorryProof
+import SciLean.Data.ArrayType
+
 namespace SciLean
 
-structure ArrayN (α : Type) (n : Nat) where
+structure ArrayN (α : Type u) (n : Nat) where
   data : Array α
   h_size : n = data.size
 
+def ArrayN.ofFn (f : Fin n → α) : ArrayN α n :=
+{
+  data := .ofFn f
+  h_size := by simp
+}
+
+def ArrayN.mapIdx {α β : Type*} (a : ArrayN α n) (f : Fin n → α → β) : ArrayN β n :=
+{
+  data := a.data.mapIdx (λ i v => f ⟨i, by have := a.2; omega⟩ v)
+  h_size := by simp[a.2]
+}
+
+def ArrayN.map {α β : Type*} (a : ArrayN α n) (f : α → β) : ArrayN β n := a.mapIdx (fun _ => f)
+
+
+instance : ArrayType (ArrayN α n) (Fin n) α where
+  ofFn := ArrayN.ofFn
+  get := fun a i => a.data.get ⟨i, by have := a.2; have := i.2; simp_all⟩
+  set := fun a i v => {
+    data := a.data.set ⟨i.1, by have := a.2; omega⟩ v
+    h_size := by have := a.2; simp_all
+  }
+  modify := fun a i f => {
+    data := a.data.modify i f
+    h_size := by have := a.2; simp_all
+  }
+  get_ofFn := by intro i; simp[ArrayN.ofFn]
+  ofFn_get := by intro f; simp[ArrayN.ofFn]
+  get_set_eq := by
+    intro a i v; simp
+  get_set_neq := by
+    intro a i j v h; simp [h]
+    sorry_proof
+  modify_set := by
+    intro a i v; simp
+    sorry_proof
 instance : GetElem (ArrayN α n) (Fin n) α (λ _ _ => True) where
-  getElem arr i _ := arr.data.get (arr.h_size ▸ i)
+  getElem arr i _ := arr.data.get ⟨i.1, by have := arr.2; omega⟩
+
+
+@[simp]
+theorem ArrayN.ofFn_get (f : Fin n → α) (i : Fin n) :
+    (ofFn f)[i] = f i := by
+  sorry_proof
+
+@[simp]
+def ArrayN.mk_get (data : Array α) (h_size : n = data.size) (i : Fin n) :
+  (ArrayN.mk data h_size)[i] = data[i] := by rfl
+
+@[simp]
+def ArrayN.get_normalize (a : ArrayN α n) (i : Fin n) :
+  have := a.2
+  a.data[i.1] = a[i] := by simp[ArrayType.get]
+
 
 instance [Inhabited α] : Inhabited (ArrayN α n) :=
   ⟨{
